\documentclass{article}
\usepackage[utf8]{inputenc}
\usepackage{parskip}
\usepackage{amsmath}
\usepackage{amssymb}
\usepackage{amsthm}
\usepackage[dvipsnames]{xcolor}

\theoremstyle{definition}
\newtheorem{definition}[subsection]{Definition}
\newtheorem{notation}[subsection]{Notation}
\newtheorem{lemma}[subsubsection]{Lemma}
\newtheorem{theorem}[subsection]{Theorem}

\title{Kandikaatopaikka}
\author{Elli Kiiski}
\date{\today}

\begin{document}
{\large
Elli Kiiski
\par
\textbf{2021 Kandikaatopaikka}
}
\vspace{0.5cm}

\section{Hardy-Wrightin todistuksen perkaamista}

\textit{G. H. Hardyn} ja \textit{E. M. Wrightin} kirjan \textit{An Introduction to the theory of numbers} sivulla 469 olevan $\phi$-funktion alarajan todistuksen läpikäyntiä.

\subsection{Määrittely: mitä todistetaan}

Aloitetaan määrittelemällä kuvaus
\begin{equation*}
    f(n)= \frac{\phi(n)e^\gamma \log\log n}{n},
\end{equation*}
missä $\gamma$ on Eulerin vakio.

Halutaan todistaa, että $\liminf f(n)=1$, mikä on yhtäpitävää sen kanssa, että $\phi$-funktion alaraja on $\frac{n}{e^\gamma \log\log n}$.

\subsection{Määrittely: miten todistetaan}

\textcolor{red}{Pitää kirjoittaa kokonaan uusiksi alkusepitykset nyt kun sigma joudutaankin ottamaan käyttöön}

Riittää löytää funktiot $F_1(t)$ ja $F_2(t)$, joille pätee
\begin{enumerate}
\label{ehdot}
    \item $\lim_{t\rightarrow \infty} F_1(t) = 1$ ja $\lim_{t\rightarrow \infty} F_2(t) = 1$
    \item $f(n) \geq F_1(\log n)$ kaikilla $n\geq 3$
    \item $f(n_j) \leq \frac{1}{F_2(j)}$ äärettömällä kasvavalla jonolla $n_2, n_3,...$
\end{enumerate}

''Tämä tarkoittaa, että on löydetty funktio $F_1(\log n)$, jonka on sama limes infimum on yksi, mutta funktio on kaikkialla suurempi kuin $f(n)$. Tällöin funktion $f(n)$ limes infimum on enintään yksi. Vastaavasti alapuolen kanssa.''
% Ilmiselvästi täytyy selittää tuo vielä jotenkin paremmin

\subsection{Todistus osa 1: $f(n) \geq F_1(\log n)$}

Olkoot $p_1,p_2,...,p_{r-\rho} \leq \log n$ ja $p_{r-\rho+1},...,p_r > \log n$ luvun $n$ alkutekijöitä. Siis luvulla $n$ on yhteensä $r$ alkutekijää, joista $\log n$:ää suurempia on $\rho$ kappaletta.

Nyt
\begin{equation}
    (\log n)^\rho < p_{r-\rho+1} \cdot p_{r-\rho+2} \cdot \cdot \cdot p_r \leq n,
\end{equation}
mistä seuraa
\begin{equation}
    \rho < \frac{\log n}{\log\log n}.
\end{equation}

Eli $\log n$:ää suurempia alkulukutekijöitä on alle $\frac{\log n}{\log\log n}$ kappaletta.
Nyt tulokaavaa käyttäen $\phi$-funktion suhde $n$:ään voidaan ilmaista seuraavasti
\begin{align}
    \frac{\phi(n)}{n} & = \prod_{i=1}^r(1-\frac{1}{p_i})\\
    & = \prod_{i=1}^{r-\rho}(1-\frac{1}{p_i}) \prod_{i=r-\rho+1}^r(1-\frac{1}{p_i})\\
    & \geq \left(\prod_{i=1}^{r-\rho}(1-\frac{1}{p_i})\right) (1-\frac{1}{\log n})^\rho\\
    & > \left(\prod_{i=1}^{r-\rho}(1-\frac{1}{p_i})\right) (1-\frac{1}{\log n})^\frac{\log n}{\log \log n}.
\end{align}

Näin ollen voidaan valita
\begin{equation*}
    F_1(t)=e^\gamma \log t \left(1-\frac{1}{t}\right)^\frac{t}{\log t} \prod_{p\leq t} \left(1-\frac{1}{p}\right),
\end{equation*}
jolloin
\begin{align*}
    F_1(\log n) & = e^\gamma \log \log n \left(1-\frac{1}{\log n}\right)^\frac{\log n}{\log \log n} \prod_{p\leq \log n} \left(1-\frac{1}{p}\right)\\
    & = e^\gamma \log \log n \left(1-\frac{1}{\log n}\right)^\frac{\log n}{\log \log n} \prod_{i=1}^{r-\rho} \left(1-\frac{1}{p}\right)\\
    & \leq \frac{\phi(n)}{n} e^\gamma \log\log n = f(n).
\end{align*}

Kuitenkin funktiolle $F_1$ pätee Mertenin kolmannen lauseen nojalla
\begin{align*}
    \lim_{t \rightarrow \infty} F_1(t) & = \lim_{t \rightarrow \infty} e^\gamma \log t \left(1-\frac{1}{t}\right)^\frac{t}{\log t} \prod_{p\leq t} \left(1-\frac{1}{p}\right)\\
    & = \lim_{t \rightarrow \infty} e^\gamma \left( 1-\frac{1}{t}\right)^\frac{t}{\log t} \left(\log t \prod_{p\leq t} \left(1-\frac{1}{p}\right) \right)\\
    & = \lim_{t \rightarrow \infty} e^\gamma \left( 1-\frac{1}{t}\right)^\frac{t}{\log t} e^{-\gamma}\\
    & = \lim_{t \rightarrow \infty} \left( 1-\frac{1}{t}\right)^\frac{t}{\log t}\\
    & = 1
\end{align*}

Täten funktion $f$ limes infimum on korkeintaan 1.

\subsection{Todistus osa 2: $f(n_j) \leq \frac{1}{F_2(j)}$}

Next, to prove the part (\ref{eq:second}), let's define
\begin{equation*}
    g(n)=\frac{\sigma(n)}{n\,e^\gamma \log\log n}
\end{equation*}
and show that $g(n_j) \geq F_2(j)$ for an infinite increasing sequence. By theorem \ref{thm:sigmafii} the desired result will follow.

Let
\begin{equation*}
    n_j=\prod_{p\leq e^j} p^j\text{, where } j\geq 2\,.
\end{equation*}

By the lemma \ref{lemma:vartheta}
\begin{equation*}
    \log n_j = \log \prod_{p\leq e^j} p^j = j \log \prod_{p\leq e^j} p = j\vartheta(e^j) \leq Aje^j\,.
\end{equation*}

Hence
\begin{equation}
\label{eq:lognj}
    \log \log n_j = \log Aje^j = \log A + \log j + \log e^j = \log A + \log j + j\,.
\end{equation}

Since $n_j$ is the product of the primes smaller than $e^j$ to the power of $j$, by the lemma \ref{lemma:sigma} we have
\begin{equation*}
    \sigma(n_j) = \prod_{p\leq e^j} \frac{p^{j+1}-1}{p-1}
\end{equation*}
and
\begin{equation}
\label{eq:signjpernj}
    \frac{\sigma(n_j)}{n_j} = \prod_{p\leq e^j} \frac{p^{j+1}-1}{(p-1)p^j} = \prod_{p\leq e^j} \frac{p^{j+1}\left(1-\frac{1}{p^{j+1}}\right)}{p^{j+1}\left(1-\frac{1}{p}\right)} = \prod_{p\leq e^j} \frac{1-\frac{1}{p^{j+1}}}{1-\frac{1}{p}}\,.
\end{equation}

Also, by the lemma \ref{lemma:zeta}
\begin{equation}
\label{eq:zetaj}
    \prod_{p\leq e^j}\left(1-\frac{1}{p^{j+1}}\right) > \prod \left(1-\frac{1}{p^{j+1}}\right) = \frac{1}{\zeta(j+1)}\,.
\end{equation}

Now we can define
\begin{equation*}
    F_2(t)=\frac{1}{e^\gamma\,\zeta(t+1)(A+t+\log t)} \prod_{p\leq e^t} \left(\frac{1}{1-\frac{1}{p}}\right)
\end{equation*}

because by combining the results (\ref{eq:lognj}), (\ref{eq:signjpernj}) and (\ref{eq:zetaj})

\begin{align*}
    F_2(j)& = \frac{1}{e^\gamma\,\zeta(j+1)(A+j+\log j)} \prod_{p\leq e^j} \left(\frac{1}{1-\frac{1}{p}}\right)\\
    & \leq \frac{1}{e^\gamma\,\log \log n_j} \prod_{p\leq e^j} \frac{1-\frac{1}{p^{j+1}}}{1-\frac{1}{p}}\\
    & = \frac{\sigma(n_j)}{n_j\,e^\gamma\,\log \log n_j} = g(n_j)\,.
\end{align*}

By the Merten's third theorem (theorem \ref{thm:mertens})
\begin{align*}
    \lim_{t \rightarrow \infty} F_2(t) & = \lim_{t \rightarrow \infty} \frac{1}{e^\gamma\,\zeta(t+1)(A+t+\log t)} \prod_{p\leq e^t} \left(\frac{1}{1-\frac{1}{p}}\right)\\
    & = \lim_{t \rightarrow \infty} \frac{e^\gamma\,\log e^t}{e^\gamma\,\zeta(t+1)(A+t+\log t)}\\
    & = \lim_{t \rightarrow \infty} \frac{t}{\zeta(t+1)(A+t+\log t)}\\
    & = \lim_{t \rightarrow \infty} \frac{t}{A+t+\log t}\\
    & = 1\,.
\end{align*}

By the theorem \ref{thm:sigmafii}
\begin{equation*}
    f(n)\,g(n) = \frac{\phi(n)\,e^\gamma \log\log n}{n} \cdot \frac{\sigma(n)}{n\,e^\gamma \log\log n} = \frac{\phi(n)\sigma(n)}{n^2}<1
\end{equation*}

and since $g(n_j) \geq F_2(j)$

\begin{equation*}
    f(n_j)\leq \frac{1}{F_2(j)}\,.
\end{equation*}


Viel semmonen johtopäätös

\section{Okei, sigma-funktio tarvitaan}

\begin{definition}{\emph{The $\sigma$-function}}

\begin{equation*}
    \sigma(n)=\sum_{d\vert n} d\,,
\end{equation*}

meaning $\sigma(n)$ is the sum of the divisors of $n$.
\end{definition}

\begin{lemma}
\label{lemma:sigma}
Let $n=p_1^{k_1}p_2^{k_2}\cdots p_r^{k_r}$ be the prime factorization of $n$, where $p_1,p_2,...,p_r$ are distinct primes. Then
\begin{equation*}
    \sigma(n)=\prod_{i=1}^r \frac{p_i^{k_i+1}-1}{p_i-1}\,,
\end{equation*}
also denoted by
\begin{equation*}
    \sigma(n) = \prod_{p\vert n} \frac{p^{k+1}-1}{p-1}\,.
\end{equation*}

\begin{proof}
Theorem 275 in \textit{Hardy \& Wright: Introduction to the Theory of Numbers}.
\end{proof}
\end{lemma}

\begin{theorem}
\label{thm:sigmafii}
\begin{equation*}
    \frac{\phi(n)\,\sigma(n)}{n^2}<1
\end{equation*}

\begin{proof}
By the Euler's product formula and lemma \ref{lemma:sigma} we get
\begin{align*}
    \phi(n)\,\sigma(n) & = n\prod_{p\vert n}\left(1-\frac{1}{p}\right) \cdot \prod_{p\vert n} \frac{p^{k+1}-1}{p-1}\\
    & = n\prod_{p\vert n}\left(1-\frac{1}{p}\right) \cdot \prod_{p\vert n} p^k \cdot \prod_{p\vert n} \frac{p-\frac{1}{p^k}}{p-1}\\
    & = n\prod_{p\vert n}\left(1-\frac{1}{p}\right) \cdot n \prod_{p\vert n}\frac{1-\frac{1}{p^{k+1}}}{1-\frac{1}{p}}\\
    & = n^2 \prod_{p\vert n} \left( \frac{1-\frac{1}{p^{k+1}}}{1-\frac{1}{p}} - \frac{1-\frac{1}{p^{k+1}}}{p-1}\right)\\
    & = n^2 \prod_{p\vert n} \frac{p-1-\frac{1}{p^k}+\frac{1}{p^{k+1}}}{p-1}\\
    & = n^2 \prod_{p\vert n} \frac{p-1-(p-1)\frac{1}{p^{k+1}})}{p-1}\\
    & = n^2 \prod_{p\vert n} \left(1-\frac{1}{p^{k+1}}\right) < n^2\,.
\end{align*}
Equivivalently
\begin{equation*}
    \frac{\phi(n)\,\sigma(n)}{n^2}<1\,.
\end{equation*}

\end{proof}
\end{theorem}

\section{Multiplikatiivisuustodistus}

Tarttetaan alkuun modulomääritelmät ja muut (jippii lisää määriteltävää ja todistettavaa)

\begin{definition}{\emph{Congruence}}

Let $m \not = 0$. We say that $a$ is congruent to $b$ modulo $m$ if $m\vert (a-b)$.\\It it denoted by
\begin{equation*}
    a \equiv b \pmod{m}\,.
\end{equation*}
\end{definition}

\begin{lemma}
Joku lemma on varmaan tarpeen
\end{lemma}

\begin{theorem}
Euler's totient function is multiplicative:
\begin{equation*}
    gcd(m,n)=1 \quad\Rightarrow\quad \phi(mn)=\phi(m)\phi(n)\,.
\end{equation*}

\begin{proof}

(Theorem 59+60 in \textit{Hardy \& Wright: Introduction to the Theory of Numbers}.)

Assume $gcd(m,n)=1$ and $a\in\{1,2,\dots,m\}$ and $b\in\{1,2,\dots,n\}$.

%First, let's show that $bm+an$ runs through a complete set of residues $\pmod mn$.

Let $C$ be a set containing all the numbers of the form $bm+an$. Since $m$ and $n$ are co-prime and $a$ and $b$ run through a complete set of residues (mod $m$) and (mod $n$) respectively, there is exactly $mn$ numbers in the set $C$.

Let $b_1m+a_1n \in C$ and $b_2m+a_2n \in C$ be congruent to each other modulo $mn$. Now
\begin{equation*}
    b_1m+a_1n \equiv b_2m+a_2n \pmod{mn}
\end{equation*}
then
\begin{equation*}
    b_1m \equiv b_2m \pmod{m} \quad \text{and} \quad a_1n \equiv a_2n \pmod{n}
\end{equation*}
and furthermore
\begin{equation*}
    b_1 \equiv b_2 \pmod{m} \quad \text{and} \quad a_1 \equiv a_2 \pmod{n}\,.
\end{equation*}
This yields $a_1 = a_2$ and $b_1 = b_2$, since $a$ and $b$ \textcolor{red}{En osaa sanoo tätä että a ja b sisältää menee vaan yhden kerran kaikki jäännökset läpi}.
Thus all of the $mn$ numbers in $C$ are incongruent to each other and therefore $C$ forms a complete residue system modulo $mn$.

Now
\begin{align*}
    gcd(bm+an,mn)=1 \quad & \Leftrightarrow \quad gcd(bm+an,m)=1\, \text{ and } \,gcd(bm+an,n)=1\\
    & \Leftrightarrow \quad gcd(an,m)=1\, \text{ and } \,gcd(bm,n)=1\\
    & \Leftrightarrow \quad gcd(a,m)=1\, \text{ and } \,gcd(b,n)=1\,,
\end{align*}
meaning 

\textcolor{red}{TÄÄ TODISTUS JOUTAA ROSKIIN}

\end{proof}

PAREMPI TODISTUS (EHKÄ)
\begin{proof}
Assume $m>1$, $n>1$ and $gcd(m,n)=1$. Consider the array
\begin{table}[!htb]
    \centering
    \begin{tabular}{ccccc}
        $0$ & $1$ & \dots & $m-2$ & $m-1$ \\
        $m$ & $m+1$ & \dots & $m+(m-2)$ & $m+(m-1)$\\
        \vdots & \vdots & \vdots & \vdots & \vdots\\
        $(n-2)m$ & $(n-2)m+1$ & \dots & $(n-2)m+(m-2)$ & $(n-2)m+(m-1)$\\
        $(n-1)m$ & $(n-1)m+1$ & \dots & $(n-1)m+(m-2)$ & $(n-1)m+(m-1)$
    \end{tabular}
\end{table}
which consists of integers from $0$ to $mn-1$, forming a complete residue system (mod $mn$).

Clearly, each row of the array forms a complete residue system (mod $m$) and all the elements of any column are congruent to each other (mod $m$). Now there are two types of columns: $\phi(n)$ columns containing only co-primes to $m$ and the rest containing none of them.

Now consider the co-prime columns. Every column forms a complete residue system (mod $n$) (\textcolor{blue}{LeVeque: chapter 3.2, theorem 3.5, p. 52}), meaning each includes $\phi(n)$ elements co-prime to $n$. Counting $\phi(n)$ elements from all the $\phi(m)$ columns we get in total $\phi(m)\phi(n)$ numbers that are relatively prime to both $m$ and $n$.

On the other hand, since $gcd(m,n)=1$, an integer $k$ is co-prime to $mn$ if and only if both $gcd(m,k)=1$ and $gcd(n,k)=1$. Hence there are $\phi(m)\phi(n)$ numbers relatively prime to $mn$. Thus by definition $\phi(mn)=\phi(m)\phi(n)$.

The case $m=1$ or $n=1$ is trivial, since $\phi(1)=1$ and thus $\phi(mn)=\phi(m)\phi(n)$.

\end{proof}

\end{theorem}

\section{Tulokaavan todistus}

Eulerin tulokaava arvon $\phi(n)$ laskemiseksi on hyvinkin tärkeä palanen eli todistetaan se nyt suoraan englanniksi niin ei tarvitse erikseen kääntää.

\subsection{Eulers's product formula}

\begin{theorem}{\emph{Euler's product formula}}

\begin{equation*}
    \phi(n) = n \prod_{p \vert n} \left(1 - \frac{1}{p}\right)
\end{equation*}

where $\prod_{p \vert n} (1 - \frac{1}{p})$ means the product over \emph{distinct} primes that divide $n$.

\begin{proof}

Assume first that $n = p^k$, where $p\in \mathbb{P}$. Now for every $x$, for which $gdc(p^k,x)>1$, holds $x=mp^{k-1}$ for some $m\in \{1,2,...,p^{k-1}\}$.

% Siis lukujen x, joille gcd(n,x) määrä on p^{k-1}

Hence
\begin{equation*}
    \phi(n)=\phi(p^k)=p^k-p^{k-1}=p^k-\frac{p^k}{p}=\left(1-\frac{1}{p}\right)p^k=\left(1-\frac{1}{p}\right)n.
\end{equation*}

Then, in the general case, assume $n=p_1^{k_1} p_2^{k_2} \cdots p_r^{k_r}=\prod_{i=1}^r p_i^{k_i}$, where $p_1,p_2,...,p_r$ are distinct primes that divide $n$ and $k_1,k_2,...,k_r$ their powers respectively. 

% Toi "their powers" ei oo hyvä, joku kertaluku tai muu käsite pitäis kaivaa siihen

Now, since $\phi$ is a multiplicative function
\begin{align*}
    \phi(n) & = \phi(p_1^{k_1} p_1^{k_1} \cdot \cdot \cdot p_r^{k_r})\\
    & = \phi(p_1^{k_1})\,\phi(p_2^{k_2}) \cdot \cdot \cdot \phi(p_r^{k_r})\\
    & = \left(1-\frac{1}{p_1}\right)p_1^{k_1} \left(1-\frac{1}{p_2}\right)p_2^{k_2} \cdot \cdot \cdot \left(1-\frac{1}{p_r}\right)p_r^{k_r}\\
    & = \prod_{i=1}^r \left(1-\frac{1}{p_i}\right) p_i^{k_i}\\
    & = n \prod_{p \vert n} \left(1 - \frac{1}{p}\right).
\end{align*}

\end{proof}

\end{theorem}

\section{Funktioita ja muita}

\begin{definition}{The zeta-function}

\begin{equation*}
    \zeta(s) = \sum_{n=1]^\infty \frac{1}{n^s}}
\end{equation*}

The zeta-funtion converges, when $s>1$.

\begin{theorem}
\label{lemma:zeta}
For all $s>1$
\begin{equation*}
    \zeta(s) = \prod_p \frac{1}{1-\frac{1}{p^s}}
\end{equation*}
\end{theorem}

\end{definition}

\begin{definition}
Von Mangoldt function

Let $p\in\mathbb{P}$ and $k\geq1$.
\begin{equation*}
    \Lambda(n) =
    \begin{cases}
    \log p \quad \text{if } n=p^k\\
    0 \quad\quad\,\,\, \text{othewise}\,.
    \end{cases}
\end{equation*}
\end{definition}

\begin{theorem}
\label{thm:lambdaf}
\begin{equation*}
    \sum_{d\vert n} \Lambda(d) = \log n\,.
\end{equation*}
\begin{proof}
Let us denote $n=\prod p^k$. Now, by definition, we have
\begin{equation*}
    \sum_{d\vert n} \Lambda(d) = \sum_{p^k\vert n} \log p\,.
\end{equation*}
We notice that as the sum runs through all combinations of primes $p$ and positive integer powers $k$ such that $p^k\vert n$, each $\log p$ occurs $k$ times. Hence
\begin{equation*}
    \sum_{p^k\vert n} \log p = \sum a \log p = \sum \log p^a = \log \prod p^a = \log n\,.
\end{equation*}
\end{proof}
\end{theorem}

\begin{lemma}
\label{lemma:lambdadd}
\begin{equation*}
    \sum_{n\leq x} \frac{\Lambda(n)}{n} = \log x + O(1)\,.
\end{equation*}
\begin{proof}
First, we have a week form of so called Striling's formula
\begin{align*}
    \sum_{n\leq x} \log n & = \int_1^x \log t\,d[t]\\
    & = [x]\log x - [x] - \log 1 + 1\\
    & = x\log x - \{x\}\log x - x + \{x\} + 1\\
    & = x\log x - x + O(\log x)\,.
\end{align*}

On the other hand, by theorem \ref{thm:lambdaf} we can deduce
\begin{equation*}
    \sum_{n\leq x} \log n = \sum_{n\leq x} \sum_{d\vert n} \Lambda(d) = \sum_{d\leq x} \Lambda(d)\,\left[\frac{x}{d}\right] = x\cdot\sum_{d\leq x} \frac{\Lambda(d)}{d} + O(\psi(x))\,,
\end{equation*}
where $\psi(x)=\sum_{d\leq x} \Lambda(d)$ \cite{HardyWright}.

Now we have
\begin{equation*}
    x\log x - x + O(\log x) = x\cdot\sum_{d\leq x} \frac{\Lambda(d)}{d} + O(\psi(x))
\end{equation*}
yielding \cite{Goldmakher} the desired result
\begin{equation*}
    \log x + O(1) = \sum_{d\leq x} \frac{\Lambda(d)}{d}\,,
\end{equation*}
when divided by $x$.

\end{proof}
\end{lemma}

\section{Merten's theorem}

\begin{lemma}
\label{lemma:mertenapu}
If $c_1, c_2,\dots$ is a sequence of real numbers such that $c_i=0$ for $i<2$ and
\begin{equation*}
    C(t) = \sum_{n\leq t} c_n
\end{equation*}
and $f(t)$ has continuous derivative for $t \geq 2 \in \mathbb{R}$, then
\begin{equation*}
    \sum_{n\leq x} c_n\,f(n) = C(x)\,f([x])-\int_2^x C(t)\,f'(t)\,dt\,.
\end{equation*}

\begin{proof}
First we observe that $C(t) = C(n)$ and $f(n)=f([t])$, when $n\leq t\leq n+1$.

We have
\begin{align*}
    \sum_{n\leq x} c_n\,f(n) & = c_1\,f(1) + c_2\,f(2) + \dots + c_n\,f(n)\\
    & =  C(1)\,f(1) + (C(2)-C(1))\,f(2) + \dots + (C(n)-C(n-1))\,f(n)\\
    & = C(1)\,(f(1)-f(2)) + C(2)\,(f(2)-f(3)) + \dots\\
    & \quad + C(n-1)\,(f(n-1)-f(n)) + C(n)\,f(n)\\
    & = \sum_{n\leq x-1} C(n)\,(f(n)-f(n+1)) + \underbrace{C(n)\,f(n)}_\text{$C(x)\,f([x])$}\,.
\end{align*}

On the other hand, since $f(t)$ is continuously differentiable when $t\geq2$ and $C(t)=0$ elsewhere, we have
\begin{equation*}
     C(n)\,(f(n)-f(n+1)) = \int_{n+1}^n C(t)\,f'(t)\,dt = -\int_n^{n+1} C(t)\,f'(t)\,dt\,.
\end{equation*}
Finally, by combining these we get
\begin{align*}
    \sum_{n\leq x} c_n\,f(n) & = C(x)\,f([x]) + \sum_{n\leq x-1} C(n)\,(f(n)-f(n+1))\\
    & = C(x)\,f([x])-\int_2^x C(t)\,f'(t)\,dt\,.
\end{align*}

\end{proof}
\end{lemma}

\begin{theorem}{\emph{Merten's theorem}}

\begin{equation*}
    \lim_{n \rightarrow \infty} \log n \prod_{p\leq n} \left(1-\frac{1}{p}\right) = e^{-\gamma}
\end{equation*}

where $\gamma$ is the Euler's constant.
% Eulerin vakio pitänee lisätä johki, tai no katotaan miten se tossa todistuksessa tulee esiin

\begin{proof}

We start by showing that for some constant $B$
\begin{equation*}
    %\lim_{n\rightarrow\infty} \left(\sum_{p\leq n}\left(\frac{1}{p}\right) - \log\log n + B\right) = 0\,,
    \sum_{p\leq n}\left(\frac{1}{p}\right) = \log\log n + B + O\left(\frac{1}{\log x}\right)
\end{equation*}
which is also know as Mertens' second theorem.

Let us use the lemma \ref{lemma:mertenapu} with a sequence, where $c_p=\frac{\log p}{p}$ with prime indices and $c_n=0$ otherwise. Now we have $C(x) = \sum_{p\leq x} \frac{\log p}{p}$.

We observe that
\begin{align*}
    \sum_{n\leq x} \frac{\Lambda(n)}{n} & = \sum_k \sum_{p^k\leq x} \frac{\log p}{p^k}\\
    & = \sum_{p\leq x} \frac{\log p}{p} + \sum_{p\leq \sqrt{x}} \frac{\log p}{p^2} + \sum_{p\leq \sqrt[3]{x}} \frac{\log p}{p^3} + \dots\\
    & < \sum_{p\leq x} \frac{\log p}{p} + \sum_p \left(\frac{1}{p^2}+\frac{1}{p^3}+\dots\right)\,\log p\\
    & = \sum_{p\leq x} \frac{\log p}{p} + \sum_p \frac{\log p}{p(p-1)}\\
    & < \sum_{p\leq x} \frac{\log p}{p} + \underbrace{ \sum_{n\geq2}^\infty \frac{\log n}{n(n-1)}}_\text{constant $A$}\\
    & = C(x) + A\,.
\end{align*}
Now, since $A$ is a constant, we get
\begin{equation*}
    C(x) = \sum_{p\leq x} \frac{\log p}{p} = \sum_{n\leq x} \frac{\Lambda(n)}{n} + O(1) = \log x + O(1)
\end{equation*}
by lemma \ref{lemma:lambdadd}.

Now, with $f(t)=\frac{1}{\log t}$, we get
\begin{align*}
    \sum_{p\leq x} \frac{1}{p} & = \sum_{p\leq x} \frac{c_p}{f(p)}\\
    & = \frac{C(x)}{\log x} + \int_2^x \frac{C(t)}{t\log^2 t}\,dt\\
    & = \frac{\log x + O(1)}{\log x} + \int_2^x \frac{\log t + O(1)}{t\log^2 t}\,dt\\
    & = 1 + \frac{O(1)}{\log x} + \int_2^x \frac{dt}{t \log t} + \int_2^x \frac{O(1)}{t \log^2 t}\,dt\\
    & = 1 + O\left(\frac{1}{\log x}\right) + \log\log x - \log\log 2 + \int_2^\infty \frac{O(1)}{t \log^2 t}\,dt - \int_x^\infty \frac{O(1)}{t \log^2 t}\,dt\\
    & = \log\log x + \underbrace{\left(\int_2^\infty \frac{O(1)}{t \log^2 t}\,dt + 1 - \log \log 2\right)}_\text{constant $B$} + O\left(\frac{1}{\log x}\right)
\end{align*}

To reach the final form of Mertens' theorem, can be shown \cite{HardyWright} that
\begin{equation*}
    B = \gamma + \sum_{p\leq n} \left(\log \left(1-\frac{1}{p}\right)+\frac{1}{p}\right)\,,
\end{equation*}
where $\gamma$ is the Euler-Masheroni constant.

However, in its extent the proof would expand outside of the scope of this thesis. Let us take the value of $B$ as given and deduce
\begin{align*}
\sum_{p\leq n} \frac{1}{p} & = \log\log x + \gamma + \sum_{p\leq n} \left(\log \left(1-\frac{1}{p}\right)+\frac{1}{p}\right) + O\left(\frac{1}{\log x}\right)\\
0 & = \log\log x + \gamma + \sum_{p\leq n} \log \left(1-\frac{1}{p}\right) + O\left(\frac{1}{\log x}\right)\\
0 & = \log\log x + \gamma + \log \prod_{p\leq n} \left(1-\frac{1}{p}\right) + O\left(\frac{1}{\log x}\right)\\
1 & = \log x + e^\gamma + \prod_{p\leq n} \left(1-\frac{1}{p}\right) + O(1)
\end{align*}

\textcolor{red}{HÄH miks tuolta ei nyt tuukaan ulos mertens heeeelp}

\textcolor{red}{KAIKKIALLA MERTENSIIN LIITTYVÄSSÄ ON NYT VIELÄ ÄKSÄT JA ÄNNÄT JA DEET SEKAISIN!!!!!}


\end{proof}

\end{theorem}

\section{Edellisestä versiosta poistettua paskaa}

\subsubsection{Are there such integers $n$ that $\phi(n) < \sqrt{n}$?}

Let's begin with $\sqrt{n}$. Is there such large number $n$ that $\phi(n) < \sqrt{n}$? When checking the values of $\phi(n)$ for smaller $n$, we see that at least with $n=6$ the statement is true, as $\phi(6)=2<\sqrt{6}$. After that, however, the values seem to be consistently above the corresponding squareroot value.

Reasonable guess would be to assume that $\sqrt{n}$ is a lower limit for $\phi(n)$ when $n \rightarrow \infty$. With more precise examination, we see that is indeed the case.

\end{document}
